\input{../template.tex}

\begin{document}

\begin{thm}{t8}{}
    On expection, how many comparisions will it make to use QUICKSELECT to find the minimum of the array. 
\end{thm}
    Using the analysis in exercise 9(see below)\ref{thm:t9}, we can get that 
    \begin{math}
        \sum_{1\leq i<j\leq n} B_{i,j,k}&= \sum_{i=1}^{k-1}\sum_{j=i+1}^{k} B_{i,j,k}+\sum_{i=k}^{n-1}\sum_{j=i+1}^{n} B_{i,j,k}\\
                                        &= k-H_k+n-(k+1)-H_{n-k+1}\\
                                        &= 1-H_1+n-2-H_n\\
                                        &= n - 2 - H_n\\
                                        &= n - \log(n) - 2 - o(1)\\
    .\end{math}

\begin{thm}{t9}{t9}
    Derive a formula for $\mathbb{E}_\pi[C(\pi, k)]$, up to additive terms of order $o(n)$. You might want to introduce $\kappa = k / n$.
\end{thm}

\begin{itemize}
    \item case $i<j\leq k$: 
        \begin{math}
            \sum_{i=1}^{k-1}\sum_{j=i+1}^{k} B_{i,j,k}&=\sum_{i=1}^{k-1}\frac{1}{k-i+1}*(k-i)\\
                                                      &=\sum_{i=1}^{k-1}(1-\frac{1}{k-i+1})=k-(1+\frac{1}{2}+\frac{1}{3}+\dots\frac{1}{k})\\
                                                      &= k - H_k
        .\end{math}
    \item case $k\leq i<j$:
        \begin{math}
            \sum_{i=k}^{n-1}\sum_{j=i+1}^{n} B_{i,j,k}&=\sum_{j=k+1}^{n}\sum_{i=k}^{j-1} B_{i,j,k}\\
                                                      &=\sum_{j=k+1}^{n}\frac{j-k}{j-k+1}\\
                                                      &=\sum_{j=k+1}^{n}(1-\frac{1}{j-k+1})\\
                                                      &=n-k+1-(1+\frac{1}{2}+\frac{1}{3}+\dots+\frac{1}{n-k+1})\\
                                                      &=n-k+1-H_{n-k+1}
        .\end{math}
\end{itemize}

\begin{itemize}
    \item case $i<k<j$:
        \begin{math}
            \sum _{i=1}^{k-1} \sum _{j=k+1}^n \frac{1}{j-i+1} &< \sum _{i=1}^{k-1} \int_{k+1}^{n+1} \frac{1}{j-i} \mathrm{d} j \\
                                              &= \sum _{i=1}^{k-1} \ln(n+1-i) - \ln(k+1-i) \\
                                              &< \int_{i=0}^{k-1} \ln(n+1-i) - \ln(k-i) \mathrm{d} i \\
                                              &= (n+1)\ln(n+1) - k\ln k - (n-k+2)\ln(n-k+2)
        .\end{math}

        On the other hand, similarly we can have
        \begin{math}
            \sum _{i=1}^{k-1} \sum _{j=k+1}^n \frac{1}{j-i+1} &> -(-k+n+2) \ln (-k+n+2)-(k+2) \ln (k+2)+(n+1) \ln (n+1)+3 \ln (3)
        .\end{math}

        The difference between the upper bound and the lower bound is $o(n)$, thus the inaccuracy is $o(n)$.

        To write this formula more simply, we have
        \begin{math}
            \sum _{i=1}^{k-1} \sum _{j=k+1}^n \frac{1}{j-i+1} = n \ln n - k \ln k - (n-k) \ln (n-k) + o(n)
        .\end{math}

        Summing three terms up, and multiply it by 2(because there are two possible orders between $i$ and $j$),
        \begin{math}
            \mathbb{E}_\pi[C(\pi,k)] &= 2(n + n\ln n - k\ln k - (n-k)\ln (n-k)) + o(n) \\
                                     &= 2(1+\ln \frac{1}{1-\kappa} + \kappa \ln \frac{1-\kappa}{\kappa})n + o(n)
        .\end{math}

\end{itemize}

\end{document}
