\usepackage{amsmath}%! Author = jinho
%! Date = 6/11/2020

% Preamble
\input{template.tex}

% Document
\begin{document}
    \begin{thm}{}{}
        Show that the three versions of Farkas Lemma presented in class are all equivalent:
        \begin{align*}
            (\neg \exists x: Ax\le b) &\iff (\exists y\ge 0 :y^{T}A=0,y^{T}b<0) &(1)\\
            (\neg \exists x\ge 0: Ax\le b) &\iff (\exists y\ge 0 :y^{T}A\ge 0,y^{T}b<0) &(2)\\
            (\neg \exists x\ge 0: Ax= b) &\iff (\exists y :y^{T}A\ge 0,y^{T}b<0)&(3)
        \end{align*}
    \end{thm}
    \begin{proof}
        $(1)\Rightarrow(3)$:

        Let $A'=\left[
        \begin{matrix}
            A \\
            -A \\
            -I
        \end{matrix}
        \right],
        b'=\left[
        \begin{matrix}
            b \\
            -b \\
            0
        \end{matrix}
        \right]$.
        Then \begin{align*}
            (\neg \exists x\ge 0: Ax= b)&\iff(\neg \exists x: Ax\le b,-Ax\le-b,-x\le 0)\\
                                        &\iff(\neg \exists x: A'x\le b') \\
                                        &\iff(\exists y'\ge 0 :y'^{T}A'=0,y'^{T}b'<0) &(\text{derived from} (1))\\
                                        &\iff(\exists y1,y2,z\ge 0:(y_{1}^{T}-y_{2}^{T})A-z=0,(y_{1}^{T}-y_{2}^{T})b<0) &(\text{Let }y'=\left[\begin{matrix} y_1 \\y_2 \\z \end{matrix}\right])\\
                                        &\iff(\exists y,z\ge 0:y^{T}A=z,y^{T}b<0) &(y=y_1-y_2) \\
                                        &\iff(\exists y :y^{T}A\ge 0,y^{T}b<0)
        \end{align*}

        $(3)\Rightarrow(2)$:

        let $A'=\left[
        \begin{matrix}
            A & I
        \end{matrix}
        \right]$.
        \begin{align*}
            (\neg \exists x\ge 0: Ax\le b)&\iff (\neg \exists x,z\ge 0:Ax+z=b) &(Ax\le b \iff \exists z\ge 0,Ax+z=b)\\
                                          &\iff (\neg \exists x'\ge 0:A'x'=b)  &(\text{let }x'=\left[ \begin{matrix} x \\ z\end{matrix} \right])\\
                                          &\iff (\exists y :y^{T}A'\ge 0,y^{T}b<0) &(\text{derived from} (3)) \\
                                          &\iff (\exists y :y^{T}A\ge 0,y\ge 0,y^{T}b<0) \\
                                          &\iff (\exists y\ge 0 :y^{T}A\ge 0,y^{T}b<0) \\
        \end{align*}

        $(2)\Rightarrow(1)$:

        Let $A'=\left[
        \begin{matrix}
            A & -A
        \end{matrix}
        \right]$.
        \begin{align*}
            (\neg \exists x: Ax\le b) &\iff (\neg \exists x_1,x_2\ge 0: A(x_1-x_2)\le b) \\
            &\iff (\neg \exists x'\ge 0: A'x'\le b) &(\text{let }x'=\left[ \begin{matrix}x_1 \\x_2  \end{matrix} \right])\\
            &\iff (\exists y\ge 0 :y^{T}A'\ge 0,y^{T}b<0) &(\text{derived from} (2)) \\
            &\iff (\exists y\ge 0 :y^{T}A\ge 0,-y^{T}A\ge 0,y^{T}b<0) \\
            &\iff (\exists y\ge 0 :y^{T}A= 0,y^{T}b<0)
        \end{align*}
    \end{proof}


\end{document}