\input{template.tex}
\begin{document}
    \begin{thm}{}{}
        Write down the dual of MCF. 
    \end{thm}

    \begin{proof}
        First, we write down MCF in terms of inequality: 
        \begin{align*}
            minimize\ &\sum_{e\in E}c(e)f(e)\\
            subject\ to\ &\sum_{e\in E:e=(u,t)}f(e)\geq 1 & \text{(corresponds to $y_t^+$ in dual form)}\\
                &\sum_{e\in E:e=(u,t)}-f(e)\geq -1 & \text{(corresponds to $y_t^-$ in dual form)}\\
                &\sum_{e\in E:e=(u,v)}f(e)-\sum_{e\in E:e=(v,w)}f(e)\geq 0,\forall v\in V\backslash\{s,t\} & \text{(corresponds to $y_v^+$ in dual form)}\\
                &\sum_{e\in E:e=(v,w)}f(e)-\sum_{e\in E:e=(u,v)}f(e)\geq 0,\forall v\in V\backslash\{s,t\} & \text{(corresponds to $y_v^-$ in dual form)}\\
        \end{align*}
        Then write down its dual LP: (Let $S=\{e\in E:e=(s,v),v\in V\}$)
        \begin{align*}
            maximize\ &y_t^+-y_t^-\\
            subject\ to\ &(y_v^+-y_v^-)-(y_u^+-y_u^-)\leq c(e),\forall e=(u,v)\in E\backslash S\\
                        &y_v^+-y_v^-\leq c(e),\forall e=(s,v)\in S
        \end{align*}
        Now let $z_u=y_u^+-y_u^-$ for all vertices $u$, it turns to be: 
        \begin{align*}
            maximize\ &z_t\\
            subject\ to\ &z_v-z_u\leq c(e),\forall e=(u,v)\in E\backslash S\\
                        &z_v\leq c(e),\forall e=(s,v)\in S
        \end{align*}
        Let $z_v'=z_v+z_s'$, for all vertices $u$ except for $s$ and the problem turns to: 
        \begin{align*}
            maximize\ &z_t'-z_s'\\
            subject\ to\ &z_v'-z_u'\leq c(e),\forall e=(u,v)\in E
        \end{align*}
    \end{proof}

    \begin{thm}{}{}
        Interpret the dual. Show that it is the LP formulation of a "natural" maximization problem on G
    \end{thm}

    \begin{proof}[Solution]
        Consider that each vertex has a potential, and for each edge $e=(u,v)$, 
        the potential of the terminal vertex $u$ is no greater than the potential of the start vertex $v$, 
        and our goal is to maximize the potential of $t$. 
    \end{proof}
\end{document}